formal-verification/Main.lean
@@ -11,8 +11,9 @@ open SemaphoreMTB (F Order)
 
 variable [Fact (Nat.Prime Order)]
 
-theorem before_deletion_tree_matches_root (DeletionIndices: Vector F 2) (PreRoot: F) (IdComms: Vector F 2) (MerkleProofs: Vector (Vector F 3) 2) (k: F -> Prop) :
-  SemaphoreMTB.DeletionProof_2_2_3_2 DeletionIndices PreRoot IdComms MerkleProofs k →
+set_option maxHeartbeats 2000000000
+theorem before_deletion_tree_matches_root (DeletionIndices: Vector F B) (PreRoot: F) (IdComms: Vector F B) (MerkleProofs: Vector (Vector F D) B) (k: F -> Prop) :
+  gDeletionProof DeletionIndices PreRoot IdComms MerkleProofs k →
   ∃out, recover_binary_zmod' out = DeletionIndices.head ∧ is_vector_binary out ∧
   MerkleTree.recover_tail poseidon₂ (Dir.create_dir_vec out) MerkleProofs.head IdComms.head = PreRoot := by
   simp [DeletionProof_looped, deletion_rounds_uncps, DeletionLoop]
@@ -20,15 +21,15 @@ theorem before_deletion_tree_matches_root (DeletionIndices: Vector F 2) (PreRoot
   apply Exists.intro
   tauto
 
-theorem after_deletion_items_are_zero (DeletionIndices: Vector F 2) (PreRoot: F) (IdComms: Vector F 2) (MerkleProofs: Vector (Vector F 3) 2) :
-  SemaphoreMTB.DeletionProof_2_2_3_2 DeletionIndices PreRoot IdComms MerkleProofs fun post_root => ∃x, recover_binary_zmod' x = DeletionIndices.last ∧ is_vector_binary x ∧
+set_option maxHeartbeats 2000000000
+theorem after_deletion_items_are_zero (DeletionIndices: Vector F B) (PreRoot: F) (IdComms: Vector F B) (MerkleProofs: Vector (Vector F D) B) :
+  gDeletionProof DeletionIndices PreRoot IdComms MerkleProofs fun post_root => ∃x, recover_binary_zmod' x = DeletionIndices.last ∧ is_vector_binary x ∧
   MerkleTree.recover_tail poseidon₂ (Dir.create_dir_vec x) MerkleProofs.last 0 = post_root := by
   -- simp [DeletionProof_2_2_3_2_uncps]
   -- simp [DeletionLoop]
   
   -- simp [SemaphoreMTB.DeletionProof_2_2_3_2]
   -- simp [DeletionRound_uncps]
-    
 
   sorry
 
